wip

Foundation/Propositional/Entailment/Corsi/F.lean
@@ -42,7 +42,23 @@ def C_trans! (h₁ : 𝓢 ⊢! φ ➝ ψ) (h₂ : 𝓢 ⊢! ψ ➝ χ) : 𝓢 �
   apply andIR! <;> assumption;
 @[grind ⇐] lemma C_trans (h₁ : 𝓢 ⊢ φ ➝ ψ) (h₂ : 𝓢 ⊢ ψ ➝ χ) : 𝓢 ⊢ φ ➝ χ := ⟨C_trans! h₁.some h₂.some⟩
 
+def CK_right_cancel! (h₁ : 𝓢 ⊢! φ ⋏ ψ ➝ χ) (h₂ : 𝓢 ⊢! ψ) : 𝓢 ⊢! φ ➝ χ := by
+  apply C_trans! ?_ h₁;
+  apply CK!_of_C!_of_C!;
+  . apply impId!;
+  . apply af! h₂;
+lemma CK_right_cancel (h₁ : 𝓢 ⊢ φ ⋏ ψ ➝ χ) (h₂ : 𝓢 ⊢ ψ) : 𝓢 ⊢ φ ➝ χ := ⟨CK_right_cancel! h₁.some h₂.some⟩
+
+def CK_right_replace! (h₁ : 𝓢 ⊢! φ ⋏ ψ ➝ χ) (h₂ : 𝓢 ⊢! ψ' ➝ ψ) : 𝓢 ⊢! φ ⋏ ψ' ➝ χ := by
+  apply C_trans! ?_ h₁;
+  apply CK!_of_C!_of_C!
+  . apply andElimL!;
+  . apply C_trans! ?_ h₂;
+    apply andElimR!;
+lemma CK_right_replace (h₁ : 𝓢 ⊢ φ ⋏ ψ ➝ χ) (h₂ : 𝓢 ⊢ ψ' ➝ ψ) : 𝓢 ⊢ φ ⋏ ψ' ➝ χ := ⟨CK_right_replace! h₁.some h₂.some⟩
+
 end Corsi
+
 
 
 end Entailment
