Foundation/Propositional/Kripke2/FTheory.lean
@@ -1,9 +1,4 @@
-import Foundation.Propositional.Formula
-import Foundation.Propositional.Entailment.Cl.Basic
-import Foundation.Vorspiel.List.Supplemental
-import Foundation.Vorspiel.Finset.Supplemental
-import Foundation.Vorspiel.Set.Supplemental
-import Foundation.Propositional.Hilbert.Corsi.Disjunctive
+import Foundation.Propositional.Hilbert.Corsi.Deduction
 import Foundation.Propositional.Kripke2.Basic
 
 namespace LO.Propositional
@@ -23,29 +18,297 @@ structure FTheory (L : Logic ℕ) where
   protected imp_closed : ∀ {φ ψ}, L ⊢ φ ➝ ψ → φ ∈ theory → ψ ∈ theory
   protected L_subset : L ⊆ theory
 
-attribute [simp] FTheory.no_bot
 
 namespace FTheory
 
--- abbrev CanonicalRel : Rel FTheory FTheory := λ T₁ T₂ => ∀ {φ ψ}, φ ➝ ψ ∈ T₁.theory → φ ∈ T₂.theory → ψ ∈ T₂.theory
+attribute [simp] FTheory.no_bot
+attribute [grind <=] FTheory.andIR FTheory.imp_closed
+
+variable {T : FTheory L} {φ ψ χ : Formula ℕ}
+
+@[simp, grind <=]
+lemma mem_of_provable [Entailment.HasAxiomVerum L] [Entailment.AFortiori L] (hφ : L ⊢ φ) : φ ∈ T.theory := by
+  apply T.imp_closed (φ := ⊤) $ af hφ;
+  apply T.L_subset;
+  apply Logic.iff_provable.mp;
+  simp;
+
+lemma mem_trans [Entailment.HasAxiomI L] (h₁ : φ ➝ ψ ∈ T.theory) (h₂ : ψ ➝ χ ∈ T.theory) : φ ➝ χ ∈ T.theory := by
+  apply T.imp_closed (axiomI (ψ := ψ));
+  apply T.andIR h₁ h₂;
+
+@[grind <=]
+lemma mem_orIntroL [Entailment.HasAxiomOrInst L] (hφ : φ ∈ T.theory) : φ ⋎ ψ ∈ T.theory := by
+  apply T.imp_closed (φ := φ);
+  . exact orIntroL;
+  . assumption;
+
+@[grind <=]
+lemma mem_orIntroR [Entailment.HasAxiomOrInst L] (hψ : ψ ∈ T.theory) : φ ⋎ ψ ∈ T.theory := by
+  apply T.imp_closed (φ := ψ);
+  . exact orIntroR;
+  . assumption;
+
+open Hilbert.Corsi in
+lemma iff_mem_CorsiDeducible {T : FTheory (Hilbert.Corsi Ax)} : φ ∈ T.theory ↔ Deduction Ax T.theory φ := by
+  constructor;
+  . intro hφ;
+    apply Deduction.ctx hφ;
+  . intro h; induction h <;> grind
 
 end FTheory
 
-variable {L : Logic ℕ} [Entailment.F L]
+
+variable {L : Logic ℕ}
 
 structure PrimeFTheory (L : Logic ℕ) extends FTheory L where
   protected prime : ∀ {φ ψ}, φ ⋎ ψ ∈ theory → φ ∈ theory ∨ ψ ∈ theory
 
-
 namespace FTheory.lindenbaum
+
+open Classical
+open Encodable
+
+variable {φ ψ χ ξ : Formula ℕ} {T : FTheory L} {hT : χ ➝ ξ ∉ T.theory}
+
+def construction (T : FTheory L) (hT : χ ➝ ξ ∉ T.theory) : ℕ → Set (Formula ℕ)
+  | 0 => { δ | χ ➝ δ ∈ T.theory }
+  | i + 1 =>
+    match (decode i) with
+    | some δ =>
+      letI T' := construction T hT i
+      if ∀ Γ : Finset (Formula _), ↑Γ ⊆ T' → Γ.conj ⋏ δ ➝ ξ ∉ T.theory then insert δ T'
+      else T'
+    | none => construction T hT i
+
+def construction_omega (T : FTheory L) (hT : χ ➝ ξ ∉ T.theory) : Set (Formula ℕ) := ⋃ i, construction T hT i
+
+lemma subset_construction_succ : construction T hT i ⊆ construction T hT (i + 1) := by
+  dsimp [construction];
+  split;
+  . split <;> tauto;
+  . tauto;
+
+lemma subset_construction_add : construction T hT i ⊆ construction T hT (i + j) := by
+  induction j with
+  | zero => simp;
+  | succ j ih =>
+    trans construction T hT (i + j);
+    . apply ih;
+    . apply subset_construction_succ;
+
+lemma monotone_construction (hij : i ≤ j) : construction T hT i ⊆ construction T hT j := by
+  obtain ⟨k, rfl⟩ := le_iff_exists_add.mp hij;
+  apply subset_construction_add;
+
+lemma mem_omega_of_mem (h : χ ➝ δ ∈ T.theory) : δ ∈ construction_omega T hT := by
+  simp only [construction_omega, Set.mem_iUnion];
+  use 0;
+  simpa [construction];
+
+lemma of_mem_construction_omega {φ : Formula ℕ} (hφ : φ ∈ construction_omega T hT) :
+  (χ ➝ φ ∈ T.theory) ∨ (∀ Γ : Finset _, ↑Γ ⊆ construction T hT (encode φ) → Γ.conj ⋏ φ ➝ ξ ∉ T.theory) := by
+  obtain ⟨i, hi⟩ := by simpa [construction_omega] using hφ;
+  induction i with
+  | zero => left; simpa [construction] using hi;
+  | succ i ih =>
+    dsimp [construction] at hi;
+    sorry;
+    /-
+    split at hi;
+    . split_ifs at hi with h;
+      . replace hi := Set.mem_insert_iff.mp hi;
+        rcases hi with (rfl | hi);
+        . right;
+          assumption;
+        . grind;
+      . grind;
+    . grind;
+    .dsimp [construction] at hi;
+    split at hi;
+    . split_ifs at hi with h;
+      . replace hi := Set.mem_insert_iff.mp hi;
+        rcases hi with (rfl | hi);
+        . sorry;
+        . grind;
+      . grind;
+    . grind;
+    split at hi;
+    -/
+
+lemma not_of_mem_construction_omega {φ : Formula ℕ}
+  {Γ : Finset (Formula ℕ)} (hΓ : ↑Γ ⊆ construction T hT (encode φ))
+  (hφ : Γ.conj ⋏ φ ➝ ξ ∈ T.theory) :
+  φ ∉ (construction_omega T hT) := by
+  simp [construction_omega, Set.mem_iUnion];
+  intro i;
+  induction i with
+  | zero =>
+    simp [construction];
+    sorry;
+  | succ i ih =>
+    simp [construction];
+    split;
+    . split_ifs with h;
+      . rename_i δ hδ;
+        by_contra hC;
+        have : δ = φ := by grind;
+        subst this;
+        apply h Γ ((show encode δ = i by sorry) ▸ hΓ) hφ;
+      . assumption
+    . assumption;
+
+lemma of_not_mem_construction_omega {φ : Formula ℕ} (hφ : φ ∉ construction_omega T hT) :
+  (χ ➝ φ ∉ T.theory) ∧ (∃ Γ : Finset (Formula _), ↑Γ ⊆ (construction T hT (encode φ)) ∧ Γ.conj ⋏ φ ➝ ξ ∈ T.theory) := by
+  simp only [construction_omega, Set.mem_iUnion, not_exists] at hφ;
+  constructor;
+  . simpa using hφ 0;
+  . have this := hφ (encode φ + 1);
+    simp only [construction, encodek] at this;
+    split_ifs at this with h;
+    . simp at this;
+    . simpa using h;
+
+
+variable [Entailment.F L]
+
+lemma construction_omega_mem_ant : χ ∈ construction_omega T hT := by
+  apply mem_omega_of_mem;
+  apply T.mem_of_provable;
+  apply impId;
+
+lemma construction_omega_not_mem_csq : ξ ∉ construction_omega T hT := by
+  simp only [construction_omega, Set.mem_iUnion, not_exists];
+  intro i;
+  induction i with
+  | zero => simpa [construction];
+  | succ i ih =>
+    contrapose! ih;
+    dsimp [construction] at ih;
+    split at ih;
+    . split_ifs at ih with h;
+      . rename_i δ hδ;
+        have := h ∅ (by tauto);
+        contrapose! this;
+        have : ξ = δ := by grind;
+        subst this;
+        apply T.mem_of_provable;
+        simp;
+      . assumption;
+    . assumption;
+
+lemma construction_omega_andClosed :
+  letI U := construction_omega T hT
+  φ ∈ U → ψ ∈ U → φ ⋏ ψ ∈ U := by
+  rintro hφ hψ;
+  by_contra hφψ;
+  replace ⟨hφψ, ⟨Γ, hΓ₁, hΓ₂⟩⟩ := of_not_mem_construction_omega hφψ;
+
+  sorry;
+
+lemma construction_omega_impClosed :
+  letI U := construction_omega T hT
+  L ⊢ φ ➝ ψ → φ ∈ U → ψ ∈ U := by
+  rintro hφψ hφ;
+  simp only [construction_omega, Set.mem_iUnion];
+  use (encode ψ) + 1;
+  simp [construction];
+  split_ifs with h;
+  . tauto;
+  . exfalso;
+    push_neg at h;
+    obtain ⟨Γ, hΓ, hΓ₂⟩ := h;
+    have hΓ₁ : (Γ.conj ⋏ φ) ➝ (Γ.conj ⋏ ψ) ∈ T.theory := T.mem_of_provable $ by
+      sorry;
+    have : (Γ.conj ⋏ φ) ➝ ξ ∈ T.theory := T.imp_closed axiomI $ T.andIR hΓ₁ hΓ₂;
+
+     sorry;
+
+lemma construction_omega_L_subset :
+  letI U := construction_omega T hT
+  L ⊆ U := by
+  intro φ hφ;
+  simp only [construction_omega, Set.mem_iUnion];
+  use (encode φ + 1);
+  simp only [construction, encodek];
+  split_ifs with h;
+  . tauto;
+  . exfalso;
+    push_neg at h;
+    obtain ⟨Γ, hΓ, h₁⟩ := h;
+    have h₂ : Γ.conj ➝ (Γ.conj ⋏ φ) ∈ T.theory := by
+      apply T.L_subset;
+      apply Logic.iff_provable.mp;
+      apply CK_of_C_of_C;
+      . exact impId;
+      . apply af;
+        exact Logic.iff_provable.mpr hφ;
+    have : Γ.conj ➝ ξ ∈ T.theory := T.mem_trans h₂ h₁;
+
+    have : Γ.conj ➝ ξ ∈ construction_omega T hT := by sorry;
+    sorry;
+
+lemma construction_omega_prime :
+  letI U := construction_omega T hT
+  φ ⋎ ψ ∈ U → φ ∈ U ∨ ψ ∈ U := by
+  rintro hφψ;
+  by_contra! hC;
+  obtain ⟨hφ, hψ⟩ := hC;
+  obtain ⟨_, ⟨Γ, hΓ₁, hΓ₂⟩⟩ := of_not_mem_construction_omega hφ;
+  obtain ⟨_, ⟨Δ, hΔ₁, hΔ₂⟩⟩ := of_not_mem_construction_omega hψ;
+
+  let m := max (encode φ) (encode ψ);
+  have : ↑(Γ ∪ Δ) ⊆ construction T hT m := by sorry;
+  have : ((Γ.conj ⋏ Δ.conj) ⋏ (φ ⋎ ψ)) ➝ ξ ∈ T.theory := by
+    apply T.imp_closed ?_ $ T.andIR hΓ₂ hΔ₂;
+    sorry;
+  sorry;
+
+lemma construction_omega_noBot :
+  letI U := construction_omega T hT
+  ⊥ ∉ U := by
+  simp [construction_omega, Set.mem_iUnion, not_exists];
+  intro i;
+  induction i with
+  | zero =>
+    simp [construction];
+    sorry;
+  | succ i ih =>
+    contrapose! ih;
+    dsimp [construction] at ih;
+    split at ih;
+    . split_ifs at ih with h;
+      . rename_i δ hδ;
+        have := h ∅ (by tauto);
+        contrapose! this;
+        have : ⊥ = δ := by grind;
+        subst this;
+        sorry;
+      . assumption;
+    . assumption;
+
+lemma construction_rel :
+  letI U := construction_omega T hT
+  (∀ φ ψ, φ ➝ ψ ∈ T.theory → φ ∈ U → ψ ∈ U) := by
+  sorry;
 
 end FTheory.lindenbaum
 
-
-lemma FTheory.lindenbaum {χ ξ : Formula _} (T : FTheory L) (hT : χ ➝ ξ ∉ T.theory) : ∃ U : PrimeFTheory L,
+open FTheory.lindenbaum in
+lemma FTheory.lindenbaum {χ ξ : Formula _} [Entailment.F L] (T : FTheory L) (hT : χ ➝ ξ ∉ T.theory) : ∃ U : PrimeFTheory L,
   (∀ φ ψ, φ ➝ ψ ∈ T.theory → φ ∈ U.theory → ψ ∈ U.theory) ∧
-  χ ∈ U.theory ∧ ξ ∉ U.theory
-   := by sorry
+  χ ∈ U.theory ∧ ξ ∉ U.theory := by
+  use {
+     theory := construction_omega T hT,
+     no_bot := construction_omega_noBot,
+     andIR := construction_omega_andClosed,
+     imp_closed := construction_omega_impClosed,
+     L_subset := construction_omega_L_subset,
+     prime := construction_omega_prime
+  };
+  constructor;
+  . apply construction_rel;
+  . exact ⟨construction_omega_mem_ant, construction_omega_not_mem_csq⟩;
 
 abbrev emptyPrimeFTheory (L : Logic _) [Entailment.F L] [Entailment.Disjunctive L] : PrimeFTheory L where
   theory := L
@@ -68,12 +331,12 @@ instance [Entailment.F L] [Entailment.Disjunctive L] : Nonempty (PrimeFTheory L)
 
 namespace Kripke2
 
-variable [Entailment.Disjunctive L]
-variable {φ ψ χ : Formula ℕ}
+variable {Ax : Axiom ℕ} {φ ψ χ : Formula ℕ}
+variable [Entailment.F L] [Entailment.Disjunctive L]
 
 open Formula.Kripke2
 
-abbrev cannonicalModel (L : Logic ℕ) [Entailment.F L] [Entailment.Disjunctive L] : Kripke2.Model where
+abbrev canonicalModel (L : Logic ℕ) [Entailment.F L] [Entailment.Disjunctive L] : Kripke2.Model where
   World := PrimeFTheory L
   Rel T U := ∀ {φ ψ}, φ ➝ ψ ∈ T.theory → φ ∈ U.theory → ψ ∈ U.theory
   Val T a := (atom a) ∈ T.theory
@@ -83,7 +346,7 @@ abbrev cannonicalModel (L : Logic ℕ) [Entailment.F L] [Entailment.Disjunctive 
     rw [←Logic.iff_provable] at hφψ;
     exact T.imp_closed hφψ hφ;
 
-lemma truthlemma {T : cannonicalModel L} : Satisfies _ T φ ↔ φ ∈ T.theory := by
+lemma truthlemma {T : canonicalModel L} : Satisfies _ T φ ↔ φ ∈ T.theory := by
   induction φ generalizing T with
   | hatom a => simp [Kripke2.Satisfies];
   | hfalsum => simp [Kripke2.Satisfies];
@@ -106,7 +369,7 @@ lemma truthlemma {T : cannonicalModel L} : Satisfies _ T φ ↔ φ ∈ T.theory 
       . apply T.imp_closed andElimL h;
       . apply T.imp_closed andElimR h;
   | himp φ ψ ihφ ihψ =>
-    suffices (∀ {U : cannonicalModel L}, T ≺ U → φ ∈ U.theory → ψ ∈ U.theory) ↔ φ ➝ ψ ∈ T.theory by
+    suffices (∀ {U : canonicalModel L}, T ≺ U → φ ∈ U.theory → ψ ∈ U.theory) ↔ φ ➝ ψ ∈ T.theory by
       simpa [Kripke2.Satisfies, ihφ, ihψ];
     constructor;
     . contrapose!;
@@ -114,7 +377,7 @@ lemma truthlemma {T : cannonicalModel L} : Satisfies _ T φ ↔ φ ∈ T.theory 
     . rintro hφψ U RTU hφ;
       apply RTU hφψ hφ;
 
-theorem provable_of_validOnCannonicalModel : (cannonicalModel L) ⊧ φ → L ⊢ φ := by
+theorem provable_of_validOncanonicalModel : (canonicalModel L) ⊧ φ → L ⊢ φ := by
   contrapose!;
   intro h;
   apply ValidOnModel.not_of_exists_world;
